cluster_config.s.dfy
@@ -1,0 +1,22 @@
+module ClusterConfig {
+
+  datatype Constants = Constants(
+    clusterSize:nat
+  ) {
+    predicate WF() {
+      && clusterSize >= 4
+    }
+
+    function F() : nat // Max faulty tolerated
+      requires WF()
+    {
+      (clusterSize - 1) / 3
+    }
+
+    function AgreementQuorum() : nat 
+      requires WF()
+    {
+      2 * F() + 1
+    }
+  }
+}
